models/simlin/Semantics.v
@@ -56,6 +56,19 @@ Section TMapSA.
       inversion H1; subst; try tauto.
   Qed.
 
+  Lemma tree_join_disjoint :
+    forall t1 t2 t, tree_join t1 t2 t ->
+      forall a b1 b2,
+        LinCCAL.TMap.find a t1 = Some b1 ->
+        LinCCAL.TMap.find a t2 = Some b2 -> False.
+  Proof.
+    induction 1; intros; auto.
+    - destruct a; simpl in *; congruence.
+    - destruct a; simpl in *; congruence.
+    - destruct a; simpl in *; eauto.
+      subst. inversion H1; subst; contradiction.
+  Qed.
+
   #[global] Instance tmap_Join : Join (LinCCAL.tmap A) := tree_join.
   #[global] Program Instance tmap_SA : SeparationAlgebra (LinCCAL.tmap A).
   Next Obligation.
@@ -97,6 +110,99 @@ Module Semantics.
   Import LTSSpec.
   Import Lang.
 
+  Definition ThreadDomain : Type := tid -> Prop.
+
+  Definition domain_equiv (A B : ThreadDomain) : Prop :=
+    forall t, A t <-> B t.
+
+  Definition domain_empty : ThreadDomain := fun _ => False.
+  Definition domain_add (t : tid) (A : ThreadDomain) : ThreadDomain :=
+    fun t' => t' = t \/ A t'.
+  Definition domain_remove (t : tid) (A : ThreadDomain) : ThreadDomain :=
+    fun t' => t' <> t /\ A t'.
+  Definition domain_union (A B : ThreadDomain) : ThreadDomain :=
+    fun t => A t \/ B t.
+  Definition domain_disjoint (A B : ThreadDomain) : Prop :=
+    forall t, A t -> B t -> False.
+
+  Definition map_domain {X} (pi : tmap X) : ThreadDomain :=
+    fun t => exists x, TMap.find t pi = Some x.
+
+  Lemma domain_equiv_refl : forall A, domain_equiv A A.
+  Proof. firstorder. Qed.
+  Lemma domain_equiv_symm : forall A B, domain_equiv A B -> domain_equiv B A.
+  Proof. firstorder. Qed.
+  Lemma domain_equiv_trans : forall A B C,
+      domain_equiv A B -> domain_equiv B C -> domain_equiv A C.
+  Proof. firstorder. Qed.
+  Lemma domain_union_comm : forall A B,
+      domain_equiv (domain_union A B) (domain_union B A).
+  Proof. firstorder. Qed.
+  Lemma domain_union_assoc : forall A B C,
+      domain_equiv (domain_union (domain_union A B) C)
+                   (domain_union A (domain_union B C)).
+  Proof. firstorder. Qed.
+  Lemma domain_union_empty_l : forall A,
+      domain_equiv (domain_union domain_empty A) A.
+  Proof. firstorder. Qed.
+  Lemma domain_union_empty_r : forall A,
+      domain_equiv (domain_union A domain_empty) A.
+  Proof. firstorder. Qed.
+
+  Lemma map_domain_empty {X} :
+    domain_equiv (map_domain (TMap.empty X)) domain_empty.
+  Proof.
+    intros t; unfold map_domain, domain_empty.
+    rewrite TMap.gempty. split; [intros [? H]; discriminate|tauto].
+  Qed.
+
+  Lemma map_domain_add {X} (pi : tmap X) t x :
+    domain_equiv (map_domain (TMap.add t x pi))
+                 (domain_add t (map_domain pi)).
+  Proof.
+    intros t'; unfold map_domain, domain_add.
+    destruct (Pos.eq_dec t' t); subst.
+    - rewrite TMap.gss. split; [tauto|intros; eauto].
+    - rewrite TMap.gso; auto. firstorder.
+  Qed.
+
+  Lemma map_domain_remove {X} (pi : tmap X) t :
+    domain_equiv (map_domain (TMap.remove t pi))
+                 (domain_remove t (map_domain pi)).
+  Proof.
+    intros t'; unfold map_domain, domain_remove.
+    destruct (Pos.eq_dec t' t); subst.
+    - rewrite TMap.grs. split; [intros [? H]; discriminate|tauto].
+    - rewrite TMap.gro; auto. firstorder.
+  Qed.
+
+  Lemma map_domain_join {X} (pi1 pi2 pi : tmap X) :
+    @join _ tmap_Join pi1 pi2 pi ->
+    domain_equiv (map_domain pi)
+                 (domain_union (map_domain pi1) (map_domain pi2)).
+  Proof.
+    intros Hj t; unfold map_domain, domain_union.
+    split.
+    - intros [x Hx].
+      pose proof (tree_join_none _ _ _ Hj t) as Hnone.
+      destruct (TMap.find t pi1) eqn:H1; [left; eauto|].
+      destruct (TMap.find t pi2) eqn:H2; [right; eauto|].
+      assert (TMap.find t pi = None) as Hout.
+      { apply (proj2 Hnone). split; auto. }
+      congruence.
+    - intros [[x Hx]|[x Hx]].
+      + exists x. eapply tree_join_increasing; eauto.
+      + exists x. eapply tree_join_increasing; [apply join_comm; exact Hj|exact Hx].
+  Qed.
+
+  Lemma map_domain_join_disjoint {X} (pi1 pi2 pi : tmap X) :
+    @join _ tmap_Join pi1 pi2 pi ->
+    domain_disjoint (map_domain pi1) (map_domain pi2).
+  Proof.
+    intros Hj t [x Hx] [y Hy].
+    eapply tree_join_disjoint; eauto.
+  Qed.
+
   Section Semantics.
     Context {E : Op.t}.
     Context {F : Op.t}.
@@ -114,6 +220,9 @@ Module Semantics.
     }.
 
     Definition ThreadPoolState : Type := tmap ThreadState.
+
+    Definition pool_domain (c : ThreadPoolState) : ThreadDomain :=
+      map_domain c.
 
     Variant ts_step (f : Sig.op F) : ThreadEvent -> State VE -> ThreadState -> State VE -> ThreadState -> Prop :=
     | ts_inv t op k s1 s2
@@ -371,29 +480,15 @@ Module Semantics.
   Section AbstractConfig.
     Context {F : Op.t} {VF : @LTS F}.
 
-    
-    Definition DomExact {A} (π1 π2 : tmap A) : Prop :=
-      forall t, TMap.find t π1 = None <-> TMap.find t π2 = None.
-      
-    Program Instance Equivalence_DomExact : Equivalence (@DomExact (@LinState F)).
-    Next Obligation. constructor; auto. Defined.
-    Next Obligation. constructor; apply H. Defined.
-    Next Obligation. constructor; unfold DomExact in *.
-      - rewrite H, H0. auto.
-      - rewrite H, H0. auto.
-    Defined.
-    
     Definition AbstractConfigProp : Type := State VF -> tmap (@LinState F) -> Prop.
 
     Record AbstractConfig : Type := mkAC {
+      ac_active : ThreadDomain;
       ac_prop :> State VF -> tmap (@LinState F) -> Prop;
       ac_nonempty : exists ρ π, ac_prop ρ π;
-      ac_domexact : forall ρ1 π1 ρ2 π2, ac_prop ρ1 π1 -> ac_prop ρ2 π2 ->
-                      DomExact π1 π2
+      ac_domain : forall ρ π, ac_prop ρ π ->
+                    domain_equiv (map_domain π) ac_active
     }.
-
-    Definition Δ_domexact (Δ1 Δ2 : AbstractConfigProp) : Prop :=
-      forall ρ1 π1 ρ2 π2, Δ1 ρ1 π1 -> Δ2 ρ2 π2 -> DomExact π1 π2.
 
     Definition ac_equiv (Δ1 Δ2 : AbstractConfig) : Prop :=
       forall ρ π, Δ1 ρ π <-> Δ2 ρ π.
@@ -410,6 +505,79 @@ Module Semantics.
     Definition ac_subset (Δ1 Δ2 : AbstractConfig) : Prop :=
       forall ρ π, Δ1 ρ π -> Δ2 ρ π.
 
+    Lemma ac_equiv_active : forall Δ1 Δ2,
+      ac_equiv Δ1 Δ2 -> domain_equiv (ac_active Δ1) (ac_active Δ2).
+    Proof.
+      intros Δ1 Δ2 Heq.
+      destruct (ac_nonempty Δ1) as [ρ [π Hposs]].
+      pose proof (ac_domain Δ1 _ _ Hposs) as Hdom1.
+      pose proof (ac_domain Δ2 _ _ (proj1 (Heq _ _) Hposs)) as Hdom2.
+      firstorder.
+    Qed.
+
+    Lemma ac_subset_active : forall Δ1 Δ2,
+      ac_subset Δ1 Δ2 -> domain_equiv (ac_active Δ1) (ac_active Δ2).
+    Proof.
+      intros Δ1 Δ2 Hsub.
+      destruct (ac_nonempty Δ1) as [ρ [π Hposs]].
+      pose proof (ac_domain Δ1 _ _ Hposs) as Hdom1.
+      pose proof (ac_domain Δ2 _ _ (Hsub _ _ Hposs)) as Hdom2.
+      firstorder.
+    Qed.
+
+    Lemma ac_find_some_iff : forall (Δ : AbstractConfig) ρ π t,
+      Δ ρ π ->
+      (ac_active Δ t <-> exists ls, TMap.find t π = Some ls).
+    Proof.
+      intros Δ ρ π t Hposs.
+      symmetry. apply ac_domain with (ρ := ρ); auto.
+    Qed.
+
+    Lemma ac_find_none_iff : forall (Δ : AbstractConfig) ρ π t,
+      Δ ρ π ->
+      (~ ac_active Δ t <-> TMap.find t π = None).
+    Proof.
+      intros Δ ρ π t Hposs.
+      rewrite ac_find_some_iff with (ρ := ρ) (π := π); auto.
+      destruct (TMap.find t π); firstorder congruence.
+    Qed.
+
+    Lemma ac_find_none_same : forall (Δ : AbstractConfig)
+      ρ1 π1 ρ2 π2 t,
+      Δ ρ1 π1 -> Δ ρ2 π2 ->
+      TMap.find t π1 = None -> TMap.find t π2 = None.
+    Proof.
+      intros Δ ρ1 π1 ρ2 π2 t H1 H2 Hnone.
+      apply (proj1 (ac_find_none_iff Δ ρ2 π2 t H2)).
+      apply (proj2 (ac_find_none_iff Δ ρ1 π1 t H1)).
+      exact Hnone.
+    Qed.
+
+    Lemma ac_find_none_equiv : forall (Δ : AbstractConfig)
+      ρ1 π1 ρ2 π2,
+      Δ ρ1 π1 -> Δ ρ2 π2 ->
+      forall t, TMap.find t π1 = None <-> TMap.find t π2 = None.
+    Proof.
+      intros Δ ρ1 π1 ρ2 π2 H1 H2 t; split; intro Hnone.
+      - exact (ac_find_none_same Δ ρ1 π1 ρ2 π2 t H1 H2 Hnone).
+      - exact (ac_find_none_same Δ ρ2 π2 ρ1 π1 t H2 H1 Hnone).
+    Qed.
+
+    Lemma AbstractConfig_ext : forall Δ1 Δ2,
+      ac_equiv Δ1 Δ2 -> Δ1 = Δ2.
+    Proof.
+      intros [A1 P1 Hn1 Hd1] [A2 P2 Hn2 Hd2] Heq; simpl in *.
+      assert (A1 = A2) as HA.
+      { apply functional_extensionality; intros t.
+        apply propositional_extensionality.
+        exact (ac_equiv_active _ _ Heq t). }
+      assert (P1 = P2) as HP.
+      { apply functional_extensionality_dep; intros ρ.
+        apply functional_extensionality_dep; intros π.
+        apply propositional_extensionality. apply Heq. }
+      subst. f_equal; apply proof_irrelevance.
+    Qed.
+
     Definition ac_empty_prop : AbstractConfigProp :=
       fun _ _ => False.
 
@@ -417,31 +585,37 @@ Module Semantics.
     | ACSingle : ac_singleton_prop ρ π ρ π.
 
     Program Definition ac_singleton ρ π : AbstractConfig :=
-      {| ac_prop := ac_singleton_prop ρ π |}.
+      {| ac_active := map_domain π;
+         ac_prop := ac_singleton_prop ρ π |}.
     Next Obligation. exists ρ, π. constructor. Qed.
-    Next Obligation.
-      inversion H; inversion H0; subst.
-      intro. reflexivity.
-    Qed.
+    Next Obligation. inversion H; subst; apply domain_equiv_refl. Qed.
+
+    Lemma ac_singleton_active : forall ρ π,
+      domain_equiv (ac_active (ac_singleton ρ π)) (map_domain π).
+    Proof. intros; apply domain_equiv_refl. Qed.
 
     Variant ac_union_prop (Δ1 Δ2 : AbstractConfigProp) : AbstractConfigProp :=
     | ACUnionLeft ρ π: Δ1 ρ π -> ac_union_prop Δ1 Δ2 ρ π
     | ACUnionRight ρ π: Δ2 ρ π -> ac_union_prop Δ1 Δ2 ρ π.
-    Program Definition ac_union (Δ1 Δ2 : AbstractConfig) {Hdomexact: Δ_domexact Δ1 Δ2} : AbstractConfig :=
-      {| ac_prop := ac_union_prop Δ1 Δ2 |}.
+    Program Definition ac_union (Δ1 Δ2 : AbstractConfig)
+      {Hactive : domain_equiv (ac_active Δ1) (ac_active Δ2)} : AbstractConfig :=
+      {| ac_active := ac_active Δ1;
+         ac_prop := ac_union_prop Δ1 Δ2 |}.
     Next Obligation.
       pose proof ac_nonempty Δ1 as [ρ [π ?]].
       exists ρ, π.
       apply ACUnionLeft; auto.
     Qed.
     Next Obligation.
-     (* eapply ac_domexact Δ1. *)
-      inversion H; inversion H0; subst.
-      - eapply (ac_domexact Δ1); eauto.
-      - eapply Hdomexact; eauto.
-      - symmetry. eapply Hdomexact; eauto.
-      - eapply (ac_domexact Δ2); eauto.
+      inversion H; subst.
+      - eapply ac_domain; eauto.
+      - eapply domain_equiv_trans; [eapply ac_domain; eauto|].
+        apply domain_equiv_symm; exact Hactive.
     Defined.
+
+    Lemma ac_union_active : forall Δ1 Δ2 Hactive,
+      domain_equiv (ac_active (@ac_union Δ1 Δ2 Hactive)) (ac_active Δ1).
+    Proof. intros; apply domain_equiv_refl. Qed.
 
     Variant ac_intersect_prop (Δ1 Δ2 : AbstractConfigProp) : AbstractConfigProp :=
     | ACIntersect ρ π: Δ1 ρ π -> Δ2 ρ π -> ac_intersect_prop Δ1 Δ2 ρ π.
@@ -451,19 +625,34 @@ Module Semantics.
         ac_inv_prop Δ t f ρ (TMap.add t (ls_inv f) π).
       
     Program Definition ac_inv (Δ : AbstractConfig) t f : AbstractConfig :=
-      {| ac_prop := ac_inv_prop Δ t f |}.
+      {| ac_active := domain_add t (ac_active Δ);
+         ac_prop := ac_inv_prop Δ t f |}.
     Next Obligation.
       destruct (ac_nonempty Δ) as [ρ [π H]].
       exists ρ, (TMap.add t0 (ls_inv f) π). constructor. auto.
     Qed.
     Next Obligation.
-      intros ?.
-      inversion H; inversion H0; subst.
-      destruct (Pos.eq_dec t1 t0); subst.
-      - do 2 rewrite PositiveMap.gss. split; discriminate.
-      - do 2 (rewrite PositiveMap.gso; auto).
-        rewrite (ac_domexact Δ _ _ _ _ Hposs Hposs0 t1).
-        reflexivity.
+      inversion H; subst.
+      eapply domain_equiv_trans; [apply map_domain_add|].
+      unfold domain_add. intros t1. rewrite (ac_domain Δ _ _ Hposs t1).
+      reflexivity.
+    Qed.
+
+    Lemma ac_inv_active : forall Δ t f,
+      domain_equiv (ac_active (ac_inv Δ t f))
+                   (domain_add t (ac_active Δ)).
+    Proof. intros; apply domain_equiv_refl. Qed.
+
+    Lemma ac_inv_find_eq : forall Δ t f ρ π,
+      ac_inv Δ t f ρ π -> TMap.find t π = Some (ls_inv f).
+    Proof. intros; inversion H; subst; apply TMap.gss. Qed.
+
+    Lemma ac_inv_find_neq : forall Δ t f ρ π t',
+      ac_inv Δ t f ρ π -> t' <> t ->
+      exists π0, Δ ρ π0 /\ TMap.find t' π = TMap.find t' π0.
+    Proof.
+      intros; inversion H; subst. eexists; split; eauto.
+      rewrite TMap.gso; auto.
     Qed.
 
     Variant ac_res_prop (Δ : AbstractConfigProp) t : AbstractConfigProp :=
@@ -471,19 +660,34 @@ Module Semantics.
         ac_res_prop Δ t ρ (TMap.remove t π).
     
     Program Definition ac_res (Δ : AbstractConfig) t : AbstractConfig :=
-      {| ac_prop := ac_res_prop Δ t |}.
+      {| ac_active := domain_remove t (ac_active Δ);
+         ac_prop := ac_res_prop Δ t |}.
     Next Obligation.
       destruct (ac_nonempty Δ) as [ρ [π H]].
       exists ρ, (TMap.remove t0 π). constructor. auto.
     Qed.
     Next Obligation.
-      intros ?.
-      inversion H; inversion H0; subst.
-      destruct (Pos.eq_dec t1 t0); subst.
-      - do 2 rewrite PositiveMap.grs. split; auto.
-      - do 2 (rewrite PositiveMap.gro; auto).
-        rewrite (ac_domexact Δ _ _ _ _ Hposs Hposs0 t1).
-        reflexivity.
+      inversion H; subst.
+      eapply domain_equiv_trans; [apply map_domain_remove|].
+      unfold domain_remove. intros t1. rewrite (ac_domain Δ _ _ Hposs t1).
+      reflexivity.
+    Qed.
+
+    Lemma ac_res_active : forall Δ t,
+      domain_equiv (ac_active (ac_res Δ t))
+                   (domain_remove t (ac_active Δ)).
+    Proof. intros; apply domain_equiv_refl. Qed.
+
+    Lemma ac_res_find_eq : forall Δ t ρ π,
+      ac_res Δ t ρ π -> TMap.find t π = None.
+    Proof. intros; inversion H; subst; apply TMap.grs. Qed.
+
+    Lemma ac_res_find_neq : forall Δ t ρ π t',
+      ac_res Δ t ρ π -> t' <> t ->
+      exists π0, Δ ρ π0 /\ TMap.find t' π = TMap.find t' π0.
+    Proof.
+      intros; inversion H; subst. eexists; split; eauto.
+      rewrite TMap.gro; auto.
     Qed.
 
     Variant ac_steps_prop (Δ : AbstractConfigProp) : AbstractConfigProp :=
@@ -491,20 +695,19 @@ Module Semantics.
         (Hpstep : poss_steps (PossOk ρ π) (PossOk ρ' π')):
         ac_steps_prop Δ ρ' π'.
 
-    Lemma poss_step_domexact : forall ρ π ρ' π',
+    Lemma poss_step_domain : forall ρ π ρ' π',
       @poss_step _ VF (PossOk ρ π) (PossOk ρ' π') ->
-      DomExact π π'.
+      domain_equiv (map_domain π) (map_domain π').
     Proof.
-      inversion 1; subst; intro;
-      (destruct (Pos.eq_dec t1 t0); subst;
-        [rewrite PositiveMap.gss
-        | rewrite PositiveMap.gso]; auto;
-        split; try congruence).
+      inversion 1; subst; intros t'; unfold map_domain.
+      all: destruct (Pos.eq_dec t' t0); subst.
+      all: try (rewrite TMap.gss; split; [intros; eauto|intros; eauto]).
+      all: rewrite TMap.gso; auto; reflexivity.
     Qed.
 
-    Lemma poss_steps_domexact : forall ρ π ρ' π',
+    Lemma poss_steps_domain : forall ρ π ρ' π',
       @poss_steps _ VF (PossOk ρ π) (PossOk ρ' π') ->
-      DomExact π π'.
+      domain_equiv (map_domain π) (map_domain π').
     Proof.
       intros.
       remember (PossOk ρ π) as p.
@@ -512,30 +715,28 @@ Module Semantics.
       revert ρ' π' Heqp'.
       apply clos_rt_rtn1 in H.
       induction H; intros; subst.
-      - inversion Heqp'; subst. reflexivity.
+      - inversion Heqp'; subst. apply domain_equiv_refl.
       - inversion H; subst;
         specialize (IHclos_refl_trans_n1 _ _ eq_refl);
-        (eapply Equivalence_Transitive; eauto;
-          intro;
-          destruct (Pos.eq_dec t1 t0); subst;
-          [rewrite PositiveMap.gss
-          | rewrite PositiveMap.gso]; auto;
-          split; intros; try congruence).
+        eapply domain_equiv_trans; eauto; eapply poss_step_domain; eauto.
     Qed.
 
     Program Definition ac_steps (Δ : AbstractConfig) : AbstractConfig :=
-      {| ac_prop := ac_steps_prop Δ |}.
+      {| ac_active := ac_active Δ;
+         ac_prop := ac_steps_prop Δ |}.
     Next Obligation.
       destruct (ac_nonempty Δ) as [ρ [π H]].
       exists ρ, π. econstructor; eauto. apply rt_refl.
     Qed.
     Next Obligation.
-      inversion H; inversion H0; subst. clear H H0.
-      apply poss_steps_domexact in Hpstep, Hpstep0.
-      pose proof (ac_domexact _ _ _ _ _ Hposs Hposs0).
-      do 2 (eapply Equivalence_Transitive; eauto).
-      symmetry. auto.
+      inversion H; subst.
+      eapply domain_equiv_trans; [apply domain_equiv_symm; eapply poss_steps_domain; eauto|].
+      eapply ac_domain; eauto.
     Qed.
+
+    Lemma ac_steps_active : forall Δ,
+      domain_equiv (ac_active (ac_steps Δ)) (ac_active Δ).
+    Proof. intros; apply domain_equiv_refl. Qed.
 
     Lemma ac_steps_refl : forall Δ, ac_subset Δ (ac_steps Δ).
     Proof.
@@ -550,20 +751,23 @@ Module Semantics.
         ac_steps_π_prop Δ t ls1 ls2 ρf Hpstep (ρf ρ) (TMap.add t ls2 (TMap.add t ls1 π)).
     
     Program Definition ac_steps_π (Δ : AbstractConfig) t ls1 ls2 ρf Hpstep : AbstractConfig :=
-      {| ac_prop := ac_steps_π_prop Δ t ls1 ls2 ρf Hpstep |}.
+      {| ac_active := ac_active Δ;
+         ac_prop := ac_steps_π_prop Δ t ls1 ls2 ρf Hpstep |}.
     Next Obligation.
       pose proof ac_nonempty Δ as [? [? ?]].
       do 2 eexists. econstructor; eauto.
     Qed.
     Next Obligation.
-      inversion H; inversion H0; subst.
-      pose proof (Hpstep _ _ Hposs).
-      pose proof (Hpstep _ _ Hposs0).
-      eapply poss_steps_domexact in H1, H2.
-      pose proof ac_domexact _ _ _ _ _ Hposs Hposs0.
-      do 2 (eapply Equivalence_Transitive; eauto).
-      symmetry. auto.
+      inversion H; subst.
+      pose proof (Hpstep _ _ Hposs) as Hsteps.
+      eapply domain_equiv_trans; [apply domain_equiv_symm; eapply poss_steps_domain; eauto|].
+      eapply ac_domain; eauto.
     Defined.
+
+    Lemma ac_steps_π_active : forall Δ t ls1 ls2 ρf Hpstep,
+      domain_equiv (ac_active (ac_steps_π Δ t ls1 ls2 ρf Hpstep))
+                   (ac_active Δ).
+    Proof. intros; apply domain_equiv_refl. Qed.
 
     Variant ac_branch_prop (Δ : AbstractConfigProp) ρ π ρ' π' : AbstractConfigProp :=
     | ACBranch
@@ -574,15 +778,23 @@ Module Semantics.
       Program Definition ac_branch (Δ : AbstractConfig) ρ π ρ' π' 
         (Hposs : Δ ρ π)
         (Hpstep : poss_steps (PossOk ρ π) (PossOk ρ' π')): AbstractConfig :=
-        {| ac_prop := ac_branch_prop Δ ρ π ρ' π' |}.
+        {| ac_active := ac_active Δ;
+           ac_prop := ac_branch_prop Δ ρ π ρ' π' |}.
       Next Obligation.
         exists ρ', π'.
         econstructor; eauto.
       Qed.
       Next Obligation.
-        inversion H; inversion H0; subst.
-        reflexivity.
+        inversion H; subst.
+        eapply domain_equiv_trans; [apply domain_equiv_symm; eapply poss_steps_domain; eauto|].
+        eapply ac_domain; eauto.
       Defined.
+
+    Lemma ac_branch_active : forall Δ ρ π ρ' π' Hposs Hpstep,
+      domain_equiv
+        (ac_active (ac_branch Δ ρ π ρ' π' Hposs Hpstep))
+        (ac_active Δ).
+    Proof. intros; apply domain_equiv_refl. Qed.
 
     Lemma ac_branch_subset_steps : forall (Δ : AbstractConfig) ρ π ρ' π' 
         Hposs Hpstep,
@@ -604,7 +816,8 @@ Module Semantics.
         Hposs Hpstep
         (oΔ' : option AbstractConfig)
         (Htrylinchoice : ac_trylin_choice Δ oΔ') : AbstractConfig :=
-      {| ac_prop := match oΔ' with
+      {| ac_active := ac_active Δ;
+         ac_prop := match oΔ' with
                     | Some Δ' => ac_union_prop Δ' (ac_branch Δ ρ π ρ' π' Hposs Hpstep)
                     | None => ac_branch Δ ρ π ρ' π' Hposs Hpstep
                     end |}.
@@ -615,23 +828,19 @@ Module Semantics.
     Qed.
     Next Obligation.
       inversion Htrylinchoice; subst; simpl in *.
-      - inversion H; inversion H0; subst.
-        + eapply (ac_domexact Δ'); eauto.
-        + apply H1 in H2.
-          inversion H2; inversion H5; subst.
-          apply poss_steps_domexact in Hpstep0, Hpstep1.
-          eapply (ac_domexact Δ) in Hposs0; eauto.
-          etransitivity; eauto.
-          symmetry. etransitivity; eauto.
-        + apply H1 in H5.
-          inversion H2; inversion H5; subst.
-          apply poss_steps_domexact in Hpstep0, Hpstep1.
-          eapply (ac_domexact Δ) in Hposs1; [|exact Hposs0].
-          etransitivity; eauto.
-          etransitivity; eauto. symmetry; auto.
-        + eapply (ac_domexact (ac_branch Δ ρ π ρ' π' Hposs Hpstep)); eauto.
-      - eapply (ac_domexact (ac_branch Δ ρ π ρ' π' Hposs Hpstep)); eauto.
+      - inversion H; subst.
+        + eapply domain_equiv_trans; [eapply ac_domain; eauto|].
+          eapply domain_equiv_trans; [apply ac_subset_active; exact H0|].
+          apply ac_steps_active.
+        + exact (ac_domain (ac_branch Δ ρ π ρ' π' Hposs Hpstep) _ _ H1).
+      - exact (ac_domain (ac_branch Δ ρ π ρ' π' Hposs Hpstep) _ _ H).
     Defined.
+
+    Lemma ac_trylin_active : forall Δ ρ π ρ' π' Hposs Hpstep oΔ' Hchoice,
+      domain_equiv
+        (ac_active (ac_trylin Δ ρ π ρ' π' Hposs Hpstep oΔ' Hchoice))
+        (ac_active Δ).
+    Proof. intros; apply domain_equiv_refl. Qed.
 
     Lemma ac_trylin_single : forall Δ ρ π ρ' π' Hposs Hstep Hnext,
       ac_equiv (ac_trylin Δ ρ π ρ' π' Hposs Hstep None Hnext) (ac_singleton ρ' π').
@@ -707,22 +916,44 @@ Module Semantics.
           ac_join_prop ac1 ac2 ρ π.
       Program Definition ac_join (ac1 ac2 : AbstractConfig)
         (Hdisjoint : ac_disjoint ac1 ac2) : AbstractConfig :=
-        {| ac_prop := ac_join_prop ac1 ac2 |}.
+        {| ac_active := domain_union (ac_active ac1) (ac_active ac2);
+           ac_prop := ac_join_prop ac1 ac2 |}.
       Next Obligation.
         destruct_disjoint Hdisjoint.
         do 2 eexists; econstructor; eauto.
       Qed.
       Next Obligation.
-        inversion H; inversion H0; subst.
-        pose proof ac_domexact _ _ _ _ _ H1 H7.
-        pose proof ac_domexact _ _ _ _ _ H2 H8.
-        clear dependent ρ0. clear dependent ρ1.
-        clear dependent ρ2. clear dependent ρ3.
-        clear dependent ρ4. clear dependent ρ5.
-        intros ?. specialize (H5 t0). specialize (H6 t0).
-        eapply tree_join_none with (a:=t0) in H4, H10.
-        tauto.
+        inversion H; subst.
+        eapply domain_equiv_trans; [eapply map_domain_join; eauto|].
+        unfold domain_union. intros t0.
+        rewrite (ac_domain ac1 _ _ H0 t0), (ac_domain ac2 _ _ H1 t0).
+        reflexivity.
       Qed.
+
+      Lemma ac_compatible_domain_disjoint : forall (ac1 ac2 : AbstractConfig),
+        ac_disjoint ac1 ac2 ->
+        domain_disjoint (ac_active ac1) (ac_active ac2).
+      Proof.
+        intros ac1 ac2 Hd.
+        destruct_disjoint Hd.
+        pose proof (map_domain_join_disjoint _ _ _ H2) as Hmap.
+        pose proof (ac_domain ac1 _ _ H) as Hdom1.
+        pose proof (ac_domain ac2 _ _ H0) as Hdom2.
+        intros t Ha1 Ha2. eapply Hmap.
+        - apply (proj2 (Hdom1 t)); exact Ha1.
+        - apply (proj2 (Hdom2 t)); exact Ha2.
+      Qed.
+
+      Lemma ac_join_active : forall (ac1 ac2 : AbstractConfig)
+        (Hd : ac_disjoint ac1 ac2),
+        domain_equiv (ac_active (ac_join ac1 ac2 Hd))
+                     (domain_union (ac_active ac1) (ac_active ac2)).
+      Proof. intros; apply domain_equiv_refl. Qed.
+
+      Lemma ac_join_active_disjoint : forall (ac1 ac2 : AbstractConfig)
+        (Hd : ac_disjoint ac1 ac2),
+        domain_disjoint (ac_active ac1) (ac_active ac2).
+      Proof. intros; eapply ac_compatible_domain_disjoint; eauto. Qed.
 
       Lemma ac_join_comm: forall ac1 ac2 Hd1 Hd2 ρ π,
         ac_join ac1 ac2 Hd1 ρ π -> ac_join ac2 ac1 Hd2 ρ π.
@@ -756,6 +987,24 @@ Module Semantics.
         fun ac1 ac2 ac => 
           exists (Hdisjoint : ac_disjoint ac1 ac2),
           ac_equiv ac (ac_join ac1 ac2 Hdisjoint).
+
+      Lemma join_ac_active : forall ac1 ac2 ac,
+        join ac1 ac2 ac ->
+        domain_equiv (ac_active ac)
+                     (domain_union (ac_active ac1) (ac_active ac2)).
+      Proof.
+        intros ac1 ac2 ac [Hd Heq].
+        eapply domain_equiv_trans; [apply ac_equiv_active; exact Heq|].
+        apply ac_join_active.
+      Qed.
+
+      Lemma join_ac_active_disjoint : forall ac1 ac2 ac,
+        join ac1 ac2 ac ->
+        domain_disjoint (ac_active ac1) (ac_active ac2).
+      Proof.
+        intros ac1 ac2 ac [Hd Heq].
+        exact (ac_join_active_disjoint ac1 ac2 Hd).
+      Qed.
 
       #[global] Program Instance ac_SA : SeparationAlgebra AbstractConfig.
       Next Obligation.
@@ -829,6 +1078,12 @@ Module Semantics.
           + apply (@unit_join _ _ _ tmap_unit).
       Qed.
 
+      Lemma ac_unit_active :
+        domain_equiv
+          (ac_active (ac_singleton ue (LinCCAL.TMap.Leaf LinState)))
+          domain_empty.
+      Proof. apply map_domain_empty. Qed.
+
       #[global] Program Instance ac_unit : SeparationAlgebraUnit AbstractConfig ac_SA :=
         {| ue := ac_singleton ue (LinCCAL.TMap.Leaf _) |}.
       Next Obligation.
@@ -837,26 +1092,16 @@ Module Semantics.
       Next Obligation.
         intros ? ? ?.
         inversion H; subst.
-        destruct n. destruct n'.
-        simpl in *.
-        assert (ac_prop0 = ac_prop1).
-        {
-          apply functional_extensionality_dep; intros ρ.
-          apply functional_extensionality_dep; intros π.
-          apply propositional_extensionality.
-          unfold ac_equiv in H0. simpl in H0.
-          rewrite H0.
-          split; intros.
-          - econstructor; eauto.
-            + constructor.
-            + apply (@join_comm _ _ tmap_SA), (@unit_join _ _ tmap_SA tmap_unit π).
+        apply AbstractConfig_ext.
+        unfold ac_equiv in *. intros ρ π.
+        rewrite H0. split; intros.
+        - econstructor; eauto.
+          + constructor.
+          + apply (@join_comm _ _ tmap_SA), (@unit_join _ _ tmap_SA tmap_unit π).
         - inversion H1; subst.
-            inversion H2; subst.
-            apply unit_spec in H4; subst.
-            apply (@unit_spec _ _ _ tmap_unit) in H5; subst; auto.
-        }
-        subst.
-        f_equal; apply proof_irrelevance.
+          inversion H2; subst.
+          apply unit_spec in H4; subst.
+          apply (@unit_spec _ _ _ tmap_unit) in H5; subst; auto.
       Defined.
     End ACSA.
 
@@ -865,7 +1110,6 @@ Module Semantics.
   Arguments AbstractConfigProp {F} VF.
   Arguments AbstractConfig {F} VF.
 
-  #[global] Existing Instance Equivalence_DomExact.
   #[global] Existing Instance Equivalence_ACEquiv.
 
   Delimit Scope ac_scope with AbstractConfig.
